thys-2019/examples/Prim/Prim_Abstract.thy
@@ -2,9 +2,10 @@ section \<open>Prim's Algorithm\<close>
 theory Prim_Abstract
 imports 
   Main 
-  Undirected_Graph
+  Undirected_Graph_Impl
   "../../sepref/IICF/IICF"
   "../../sepref/IICF/Impl/IICF_Array_of_Array_List"
+  "../../sepref/IICF/Impl/Heaps/IICF_Impl_Heapmap"
 begin
 
 (* TODO: Move *)
@@ -29,10 +30,6 @@ begin
   lemma f_upd_same_eq_iff[simp]: "f(x:=y) = f(x:=y') \<longleftrightarrow> y=y'" by (auto simp: fun_eq_iff)
   lemma ins_eq_set_memD:  "insert x S = S' \<Longrightarrow> x\<in>S'" by blast
 
-  (* TODO: Move *)
-  lemma card2_eq: "card e = 2 \<longleftrightarrow> (\<exists>u v. u\<noteq>v \<and> e={u,v})"
-    by (auto simp: eval_nat_numeral card_Suc_eq)
-  
 
 text \<open>Restructuring refinement of a while loop: The concrete 
   loop does an initial iteration, which is invisible on the abstract level.
@@ -976,7 +973,6 @@ end
 
 subsection \<open>Refinement of Inner Foreach Loop\<close>
 
-definition "mop_wgraph_adjs g w u \<equiv> SPEC (\<lambda>adjs. set adjs = {(v,d). (u,v)\<in>edges g \<and> w {u,v} = d})"
 
 
 context Prim2 begin
@@ -1132,416 +1128,321 @@ context Prim2 begin
     apply (refine_rcg peek_min_refine Qpm_delete_refine)
     by (auto simp: Qpm_init_refine init\<pi>_def Qpm_is_empty_refine in_br_conv)
     
-    
-    
-    
-        
 end
 
 (* TODO: Move *)
-subsection \<open>Doubleton Set to Pair\<close>
-definition "epair e = (if card e = 2 then Some (SOME (u,v). e={u,v}) else None)"
-
-lemma epair_eqD: "epair e = Some (x,y) \<Longrightarrow> (x\<noteq>y \<and> e={x,y})"
-  apply (cases "card e = 2")
-  unfolding epair_def
-  apply simp_all
-  apply (clarsimp simp: card_Suc_eq eval_nat_numeral doubleton_eq_iff)
-  by (smt case_prodD case_prodI someI)
-  
-lemma epair_not_sng[simp]: "epair e \<noteq> Some (x,x)"  
-  by (auto dest: epair_eqD)
-
-lemma epair_None[simp]: "epair {a,b} = None \<longleftrightarrow> a=b" 
-  unfolding epair_def by (auto simp: card2_eq) 
-
-lemma epair_cases:
-  obtains (edge) u v where "e={u,v}" "u\<noteq>v" "epair e = Some (u,v)"
-        | (no_edge) "card e \<noteq> 2" "epair e = None"
-  by (metis card2_eq epair_None epair_eqD not_Some_eq2)
-
-
-type_synonym ('v,'w) wugraph1 = "'v \<Rightarrow> ('v\<rightharpoonup>'w)"
-
-definition wu1_invar :: "('v,'w) wugraph1 \<Rightarrow> bool" 
-  where "wu1_invar g1 \<equiv> 
-      (\<forall>u. g1 u u = None) 
-    \<and> (\<forall>u v w. g1 u v = Some w \<longrightarrow> g1 v u = Some w)
-    \<and> finite { (u,v). g1 u v \<noteq> None }"
-definition wu1_\<alpha>E :: "('v,'w) wugraph1 \<Rightarrow> ('v\<times>'v) set" where "wu1_\<alpha>E g1 \<equiv> { (u,v). g1 u v \<noteq> None }"
-definition wu1_\<alpha>g :: "('v,'w) wugraph1 \<Rightarrow> 'v ugraph" where "wu1_\<alpha>g g1 \<equiv> graph {} (wu1_\<alpha>E g1)"
-
-definition wu1_\<alpha>w :: "('v,'w::zero) wugraph1 \<Rightarrow> 'v set \<Rightarrow> 'w" where 
-  "wu1_\<alpha>w g1 e \<equiv> case epair e of Some (u,v) \<Rightarrow> the_default 0 (g1 u v) | None \<Rightarrow> 0"
-
-lemma wu1_invar_alt: "wu1_invar g1 \<equiv> 
-      (\<forall>u. g1 u u = None) 
-    \<and> (\<forall>u v w. g1 u v = Some w \<longrightarrow> g1 v u = Some w)
-    \<and> finite (wu1_\<alpha>E g1)"  
-  unfolding wu1_invar_def wu1_\<alpha>E_def by simp
-  
-definition wu1_empty :: "('v,'w) wugraph1" where "wu1_empty \<equiv> \<lambda>_ _. None"
-definition wu1_ins_edge :: "'v\<times>'v \<Rightarrow> 'w \<Rightarrow> ('v,'w) wugraph1 \<Rightarrow> ('v,'w) wugraph1 nres"
-  where "wu1_ins_edge \<equiv> \<lambda>(u,v) w g. doN {
-    ASSERT (v \<notin> dom (g u));
-    gu \<leftarrow> mop_map_update v w (g u);
-    let g = g(u:=gu);
-    ASSERT (u \<notin> dom (g v));
-    gv \<leftarrow> mop_map_update u w (g v);
-    let g = g(v:=gv);
-    RETURN g
-  }"
-definition wu1_adjs :: "'v \<Rightarrow> ('v,'w) wugraph1 \<Rightarrow> ('v\<times>'w) list nres" 
-  where "wu1_adjs u g1 \<equiv> SPEC (\<lambda>xs. distinct xs \<and> set xs = {(v,w). g1 u v = Some w})"
+lemma WHILEIT_refine_new_invar':
+  assumes R0: "I' x' \<Longrightarrow> (x,x')\<in>R"
+  assumes INV0: "\<lbrakk> I' x'; (x,x')\<in>R \<rbrakk> \<Longrightarrow> I x"
+  assumes COND_REF: "\<And>x x'. \<lbrakk> (x,x')\<in>R; I x; I' x' \<rbrakk> \<Longrightarrow> b x = b' x'"
+  assumes STEP_REF: 
+    "\<And>x x'. \<lbrakk> (x,x')\<in>R; b x; b' x'; I x; I' x' \<rbrakk> \<Longrightarrow> f x \<le> \<Down>R (f' x')"
+  assumes STEP_INV: 
+    "\<And>x x'. \<lbrakk> (x,x')\<in>R; b x; b' x'; I x; I' x' \<rbrakk> \<Longrightarrow> f x \<le>\<^sub>n SPEC I"
+  shows "WHILEIT I b f x \<le>\<Down>R (WHILEIT I' b' f' x')"
+  apply (rule WHILEIT_refine_genR[where 
+    I=I and I'=I' and x'=x' and x=x and R=R and b=b and b'=b' and f'=f' and f=f
+    and R'="{ (c,a). (c,a)\<in>R \<and> I c }"
+    ])
+  using assms STEP_INV[THEN leofD[rotated]]
+  by (auto intro: add_invar_refineI)
   
 
-lemma wu1_empty_refine[simp]:
-  "wu1_invar wu1_empty"  
-  "wu1_\<alpha>g wu1_empty = graph_empty"
-  "wu1_\<alpha>w wu1_empty = (\<lambda>_. 0)"
-  by (auto 
-    simp: wu1_invar_def wu1_empty_def wu1_\<alpha>g_def wu1_\<alpha>E_def wu1_\<alpha>w_def[abs_def]
-    simp: fun_eq_iff split: option.splits
-    )
-  
-lemma wu1_irrefl[simp]: "wu1_invar g \<Longrightarrow> g u u = None" by (auto simp: wu1_invar_def)
-lemma wu1_sym: "wu1_invar g \<Longrightarrow> g u v = g v u" 
-  apply (cases "g u v"; cases "g v u"; simp)
-  unfolding wu1_invar_def
-  apply (metis option.simps(3))
-  apply (metis option.simps(3))
-  apply (metis option.simps(1))
-  done
 
-lemma wu1_finite[simp, intro]: "wu1_invar g \<Longrightarrow> finite (wu1_\<alpha>E g)"
-  unfolding wu1_invar_alt by auto
-  
-lemma wu1_edges_aux: "wu1_invar g \<Longrightarrow> edges (graph {} (wu1_\<alpha>E g)) = wu1_\<alpha>E g"
-  apply (simp add: edges_graph)
-  apply (auto simp: wu1_\<alpha>E_def wu1_sym)
-  done
-  
-lemma wu1_edges_aux2: "wu1_invar g \<Longrightarrow> edges (wu1_\<alpha>g g) = wu1_\<alpha>E g"
-  unfolding wu1_\<alpha>g_def by (simp add: wu1_edges_aux)
 
+
+
+locale Prim5 = Prim2 w g r for w :: "nat set \<Rightarrow> nat" and g r + 
+  fixes g2 :: "nat wugraph2" 
+begin
+
+  definition "N \<equiv> wu2_max g2"
+
+  (*definition "upd_Q\<pi>_loop3 u Q \<pi> \<equiv> doN {
+      num_adjs \<leftarrow> wu2_adjs_len u g2;
+      nfoldli [0..<num_adjs] (\<lambda>_. True)
+       (\<lambda>i (Q, \<pi>). doN {
+             vd \<leftarrow> wu2_adjs_nth u i g2;
+             case vd of (v, d) \<Rightarrow>
+               if v = r then RETURN (Q, \<pi>)
+               else (case (op_map_lookup v Q, op_map_lookup v \<pi>) of (None, None) \<Rightarrow> RETURN (Q(v \<mapsto> d), \<pi>(v \<mapsto> u))
+                    | (None, Some xa) \<Rightarrow> RETURN (Q, \<pi>)
+                    | (Some d', x) \<Rightarrow> if d < d' then RETURN (Q(v \<mapsto> d), \<pi>(v \<mapsto> u)) else RETURN (Q, \<pi>))
+              
+           })
+       (Q, \<pi>)
+    }"*)
+
+  definition "upd_Q\<pi>_loop3 u Q \<pi> \<equiv> doN {
+      num_adjs \<leftarrow> wu2_adjs_len u g2;
+      nfoldli [0..<num_adjs] (\<lambda>_. True)
+       (\<lambda>i (Q, \<pi>). doN {
+            vd \<leftarrow> wu2_adjs_nth u i g2;
+            case vd of (v, d) \<Rightarrow>
+              if v = r then RETURN (Q, \<pi>)
+              else doN {
+                ASSERT (v<N);
+                if op_map_contains_key v Q then
+                  if d < op_map_the_lookup v Q then RETURN (Q(v \<mapsto> d), \<pi>(v \<mapsto> u)) else RETURN (Q, \<pi>)
+                else
+                  if op_map_contains_key v \<pi> then RETURN (Q,\<pi>) else RETURN (Q(v \<mapsto> d), \<pi>(v \<mapsto> u))
+            }
+          })
+       (Q, \<pi>)
+    }"
+    
+    
+    
+  definition "prim5 \<equiv> doN {
+    Q \<leftarrow> HM.mop_hm_empty (wu2_max g2);
+    ASSERT (r<N);
+    let Q = op_map_update r 0 Q;
+    \<pi> \<leftarrow> mop_am_custom_empty (wu2_max g2);
+    WHILEIT (\<lambda>(Q,\<pi>). dom Q \<subseteq> {0..<N})
+      (\<lambda>(Q,\<pi>). \<not>op_map_is_empty Q) 
+      (\<lambda>(Q,\<pi>). doN { 
+        (u,_) \<leftarrow> mop_pm_peek_min id Q;
+        (Q,\<pi>) \<leftarrow> upd_Q\<pi>_loop3 u Q \<pi>;
+        ASSERT (u<N);
+        Q \<leftarrow> mop_map_delete u Q;
+        RETURN (Q,\<pi>) 
+      })
+      (Q,\<pi>)
+    }
+    "
+
+  context
+    assumes G_REL: "(g2,(g,w))\<in>wu_rel N"
+    assumes R_ND: "r<N"
+  begin    
+    
+    private lemma wu2_adjs_nth_bound: "wu2_adjs_nth u i g2 \<le>\<^sub>n SPEC (\<lambda>(v,d). v<N)"
+      unfolding wu2_adjs_nth_def
+      apply refine_vcg
+      using G_REL
+      unfolding wu_rel_def wu2_invar_def
+      apply (auto simp: Let_def)
+      by (metis atLeastLessThan_iff fst_image_mp nth_mem)
   
-lemma wu1_\<alpha>E_ins_aux:
-  assumes "wu1_invar g" "(u,v)\<notin>edges (wu1_\<alpha>g g)" "u\<noteq>v"
-  shows "wu1_\<alpha>E (g(u := g u(v \<mapsto> w), v := g v(u \<mapsto> w))) = {(u,v),(v,u)} \<union> wu1_\<alpha>E g"  
-  using assms
-  unfolding wu1_\<alpha>g_def
-  apply (simp add: wu1_edges_aux)
-  unfolding wu1_\<alpha>E_def
-  by (auto split!: if_splits)
   
+    method Q\<pi>3_refine = (rule bind_refine; Q\<pi>3_refine | rule nfoldli_refine)?
+    lemma upd_Q\<pi>_loop3_refine[refine]:
+      assumes "(ui,u)\<in>Id" "(Qi,Q)\<in>Id" "(\<pi>i,\<pi>)\<in>Id" "u<N"
+      shows "upd_Q\<pi>_loop3 ui Qi \<pi>i \<le>\<Down> Id (upd_Q\<pi>_loop2 u Q \<pi>)"
+      apply (simp add: assms(1-3)[simplified])
+      apply (rule order_trans[rotated])
+      unfolding upd_Q\<pi>_loop2_def
+      apply (rule iterate_adjs_refine_aux[OF G_REL])
+      apply fact
+      unfolding upd_Q\<pi>_loop3_def
+      apply (rule refine_IdD)
+      (* TODO: A more flexible refine_rcg tactic might save us from this manual rule applications *)
+      apply Q\<pi>3_refine
+      apply refine_dref_type
+      supply conc_Id[simp del]
+      apply (clarsimp_all simp: refine_IdI[OF order_refl])
+      apply (rule bind_refine')
+      apply (rule refine_IdI[OF order_refl])
+      apply (clarsimp split del: if_split)
+      apply (rule if_refine)
+      apply simp
+      apply simp
+      apply (rule ASSERT_refine_left)
+      subgoal using wu2_adjs_nth_bound by (auto simp: pw_leof_iff)
+      subgoal by (auto simp: pw_le_iff refine_pw_simps split: option.splits)
+      done
+      
+    lemma N_len_eq: "N=length g2" using G_REL by (auto simp: wu_rel_def Let_def)
+    
+    lemma prim5_refine: "prim5 \<le>\<Down>Id prim4"  
+      unfolding prim4_def prim5_def Let_def
+      apply (rewrite in "_ \<le> \<Down>_ \<hole>" WHILET_def)
+      apply (simp del: conc_Id)
+      apply (refine_vcg bind_refine' WHILEIT_refine_new_invar')
+      
+      apply (clarsimp_all split: if_splits simp: R_ND)
+      subgoal by auto
+      subgoal by auto
+      subgoal        
+        unfolding upd_Q\<pi>_loop3_def wu2_adjs_len_def wu2_adjs_nth_def
+        apply (refine_vcg nfoldli_leof_rule[where I="\<lambda>_ _ (Q,\<pi>). dom Q \<subseteq> {0..<N}"])
+        apply (clarsimp_all split: if_splits)
+        apply (auto simp: N_len_eq)
+        (*apply (auto simp: wu2_invar_def) 
+        by (metis (mono_tags, hide_lams) atLeastLessThan_iff img_fst nth_mem subsetD)
+        *)
+        done
+      done
+
+  end    
+end    
+
+lemma Nil_eq_upt_conv: "[] = [l..<h] \<longleftrightarrow> l\<ge>h"
+  by (metis upt_eq_Nil_conv zero_le)
+
+lemma eq_upt_Cons_conv: "ll#xs = [l..<h] \<longleftrightarrow> (l<h \<and> ll=l \<and> xs = [l+1..<h])"
+  by (metis upt_eq_Cons_conv)
   
-lemma wu1_ins_edge_refine[simp]:
-  assumes "wu1_invar g" "(u,v)\<notin>edges (wu1_\<alpha>g g)" "u\<noteq>v"
-  shows "wu1_ins_edge (u,v) w g \<le> SPEC (\<lambda>g'. 
-      wu1_invar g'
-    \<and> wu1_\<alpha>g g' = ins_edge (u,v) (wu1_\<alpha>g g)
-    \<and> wu1_\<alpha>w g' = (wu1_\<alpha>w g)({u,v}:=w)
-  )"
-  unfolding wu1_ins_edge_def
-  apply (refine_vcg)
-  apply (simp_all add: \<open>u\<noteq>v\<close>[symmetric] split: if_splits)
-  apply (all \<open>(elim conjE)?;(hypsubst)?\<close>)
+(* TODO: Move! Ultimately, we want sepref-rules and a foreach-statement *)  
+lemma nfoldli_upt_by_while:
+  "nfoldli [l..<h] c f \<sigma> =
+  doN { (_,\<sigma>)\<leftarrow>WHILET (\<lambda>(i,\<sigma>). i<h \<and> c \<sigma>) (\<lambda>(i,\<sigma>). doN { \<sigma> \<leftarrow> f i \<sigma>; ASSERT (i<h); RETURN (i+1,\<sigma>) }) (l,\<sigma>); RETURN \<sigma> }
+  "
+proof (induction "[l..<h]" arbitrary: l \<sigma>)
+  case Nil thus ?case
+    apply (simp add: Nil_eq_upt_conv)
+    apply (rewrite WHILET_unfold)
+    by simp
+next
+  case (Cons ll xs)
   
-  subgoal 
-    using assms(2)
-    apply (auto simp: \<open>wu1_invar g\<close> wu1_edges_aux2)
-    by (auto simp: wu1_\<alpha>E_def)
-  subgoal 
-    using assms(1) assms(3) wu1_sym by fastforce
-  subgoal
-    using \<open>u\<noteq>v\<close>
-    unfolding wu1_invar_alt wu1_ins_edge_def
-    by (auto simp: \<open>wu1_invar g\<close> wu1_sym wu1_\<alpha>E_ins_aux[OF assms(1-3)])
-  subgoal
-    unfolding wu1_\<alpha>g_def wu1_ins_edge_def
-    apply (simp add: wu1_\<alpha>E_ins_aux[OF assms(1-3)])
-    apply (rewrite graph_eq_iff; simp add: nodes_graph edges_graph edges_ins_edge \<open>wu1_invar g\<close>)
-    by auto
-  subgoal
-    unfolding wu1_\<alpha>w_def wu1_ins_edge_def
-    apply (rule ext)
-    subgoal for e by (cases e rule: epair_cases) auto
+  from Cons.hyps(2)[symmetric] have [simp]: "l<h" and [simp]: "ll=l" "[l..<h] = l#[l+1..<h]" "xs=[l+1..<h]"
+    by (auto simp: upt_eq_Cons_conv)
+  
+  note IH = Cons.hyps(1)[of "Suc l",simplified,abs_def]  
+    
+  from Cons.hyps(2) show ?case
+    apply (rewrite WHILET_unfold)
+    apply (auto simp add: IH)
     done
-  done  
-
-  
-lemma wu1_adjs_refine:  
-  assumes "wu1_invar g"
-  shows "wu1_adjs u g \<le> mop_wgraph_adjs (wu1_\<alpha>g g) (wu1_\<alpha>w g) u"
-  apply (simp add: wu1_edges_aux2[OF assms] wu1_adjs_def mop_wgraph_adjs_def)
-  apply (auto simp: wu1_\<alpha>w_def wu1_\<alpha>E_def)
-  apply (auto 
-    split: option.split 
-    simp: doubleton_eq_iff wu1_irrefl[OF assms] wu1_sym[OF assms]
-    dest!: epair_eqD)
-  done
-  
-(*      
-lemma wu1_adjs_refine[simp]:  
-  assumes "wu1_invar g"
-  shows "wu1_adjs u g = {(v,wu1_\<alpha>w g {u,v}) | v. (u,v)\<in>edges (wu1_\<alpha>g g)}"
-  apply (simp add: wu1_edges_aux2[OF assms] wu1_adjs_def)
-  apply (auto simp: wu1_\<alpha>w_def wu1_\<alpha>E_def)
-  apply (auto 
-    split: option.split 
-    simp: doubleton_eq_iff wu1_irrefl[OF assms] wu1_sym[OF assms]
-    dest!: epair_eqD)
-  done
-*)  
-
-type_synonym 'w wugraph2 = "(nat\<times>'w) list list"
-
-definition wu2_invar :: "'w wugraph2 \<Rightarrow> bool" 
-  where "wu2_invar xss \<equiv> 
-    let N=length xss in 
-      \<forall>xs\<in>set xss. distinct (map fst xs) \<and> fst`set xs \<subseteq> {0..<N}"
-
-definition wu2_\<alpha> :: "'w wugraph2 \<Rightarrow> (nat,'w) wugraph1"
-  where "wu2_\<alpha> xss \<equiv> \<lambda>u. if u<length xss then map_of (xss!u) else Map.empty"
-
-definition wu2_empty :: "nat \<Rightarrow> 'w wugraph2" where "wu2_empty N \<equiv> replicate N []"
-definition wu2_ins_edge :: "nat \<times> nat \<Rightarrow> 'w \<Rightarrow> 'w wugraph2 \<Rightarrow> 'w wugraph2 nres" where
-  "wu2_ins_edge \<equiv> \<lambda>(u,v) w xss. doN {
-    ASSERT (u<length xss \<and> length (xss!u) < length xss);
-    xss \<leftarrow> mop_list_list_push_back xss u (v,w);
-    ASSERT (v<length xss \<and> length (xss!v) < length xss);
-    xss \<leftarrow> mop_list_list_push_back xss v (u,w);
-    RETURN xss
-  }"
-
-definition wu2_adjs :: "nat \<Rightarrow> 'w wugraph2 \<Rightarrow> (nat\<times>'w) list nres" where
-  "wu2_adjs u xss \<equiv> doN { ASSERT (u<length xss); RETURN (xss!u) }"
-  
-lemma wu2_empty_refine[simp]:
-  "wu2_invar (wu2_empty N)"  
-  "wu2_\<alpha> (wu2_empty N) = wu1_empty"
-  unfolding wu2_invar_def wu2_empty_def wu2_\<alpha>_def wu1_empty_def
-  by auto
-
-(* TODO: Move *)  
-lemma distinct_bounded_list_add_bound:
-  assumes D: "distinct xs"  
-  assumes SS: "set xs \<subseteq> {0..<N}"
-  assumes NI: "x<N" "x\<notin>set xs"
-  shows "length xs < N"
-proof -
-  from SS NI have "set xs \<subseteq> {0..<N} - {x}" by auto
-  from card_mono[OF _ this] have "card (set xs) < N" using NI by auto
-  with distinct_card[OF D] show ?thesis by simp
+    
 qed    
-  
-lemma wu2_ins_edge_bound_aux:
-  assumes "wu2_invar xss" "u<length xss" "v<length xss" "wu2_\<alpha> xss u v = None"  
-  shows "length (xss!u) < length xss"
-proof -
-  have "length (map fst (xss!u)) < length xss"
-    apply (rule distinct_bounded_list_add_bound[OF _ _ \<open>v<length xss\<close>])
-    using assms
-    unfolding wu2_invar_def wu2_\<alpha>_def
-    by auto
-  thus ?thesis by auto
-qed
-  
-lemma wu2_ins_edge_refine: 
-  "\<lbrakk>(xss,g)\<in>br wu2_\<alpha> wu2_invar; u<length xss; v<length xss\<rbrakk> \<Longrightarrow> wu2_ins_edge (u,v) w xss \<le>\<Down>(br wu2_\<alpha> wu2_invar) (wu1_ins_edge (u,v) w g)"
-  unfolding wu2_ins_edge_def wu1_ins_edge_def
-  apply (auto simp: pw_le_iff refine_pw_simps in_br_conv intro: wu2_ins_edge_bound_aux)
-  apply (auto 
-    elim!: in_set_upd_cases 
-    simp: map_add_find_left wu2_invar_def wu2_\<alpha>_def fun_eq_iff 
-    split!: if_splits)
-  subgoal
-    by (meson atLeastLessThan_iff img_fst nth_mem subsetD)
-  subgoal
-    by (meson atLeastLessThan_iff img_fst nth_mem subsetD) 
-  subgoal
-    using atLeastLessThan_iff by blast
-  done  
-  
-  
-lemma wu2_adjs_refine:
-  "\<lbrakk>(xss,g)\<in>br wu2_\<alpha> wu2_invar; u<length xss\<rbrakk> \<Longrightarrow> wu2_adjs u xss \<le> wu1_adjs u g"
-  unfolding wu2_adjs_def wu1_adjs_def
-  apply refine_vcg
-  apply (clarsimp_all simp: pw_le_iff refine_pw_simps in_br_conv)
-  apply (auto simp: wu2_invar_def wu1_adjs_def wu2_\<alpha>_def)
-  using distinct_mapI nth_mem by blast
-  
-definition wu2_adjs_len :: "nat \<Rightarrow> 'w wugraph2 \<Rightarrow> nat nres" where
-  "wu2_adjs_len u xss \<equiv> mop_list_list_llen xss u"
-  
-definition wu2_adjs_nth :: "nat \<Rightarrow> nat \<Rightarrow> 'w wugraph2 \<Rightarrow> (nat\<times>'w) nres" where
-  "wu2_adjs_nth u i xss \<equiv> mop_list_list_idx xss u i"
 
 
-definition "wu_rel N \<equiv> {(g2,(g,w)). let g1 = (wu2_\<alpha> g2) in g = wu1_\<alpha>g g1 \<and> w = wu1_\<alpha>w g1 \<and> wu1_invar g1 \<and> wu2_invar g2 \<and> length g2=N }"
+find_theorems WHILET nfoldli
 
-lemma wu_empty_refine: "(wu2_empty N, (graph_empty, \<lambda>_. 0)) \<in> wu_rel N"
-  apply (auto simp: wu_rel_def)
-  by (simp add: wu2_empty_def)
+   
+abbreviation "snat32_assn \<equiv> snat_assn' TYPE(32)"
+abbreviation "snat64_assn \<equiv> snat_assn' TYPE(64)"
+abbreviation "wu3_64_assn \<equiv> wu3_assn' TYPE(64) TYPE(64)"
 
-lemma wu_ins_edge_refine: 
-  assumes "(ui,u)\<in>Id" "(vi,v)\<in>Id" "(di,d)\<in>Id" "u<N" "v<N" "(g2,(g,w))\<in>wu_rel N"
-  assumes "(u,v)\<notin>edges g" "u\<noteq>v"
-  shows "wu2_ins_edge (ui,vi) di g2 \<le> \<Down>(wu_rel N) (RETURN (ins_edge (u,v) g, w({u,v}:=d)))"
-  using assms
-  using wu2_ins_edge_refine[of "g2" "wu2_\<alpha> g2" u v d] 
-  using wu1_ins_edge_refine[of "wu2_\<alpha> g2" u v d]
-  apply (auto simp: wu_rel_def pw_le_iff refine_pw_simps Let_def in_br_conv)
-  apply (auto simp: wu2_ins_edge_def refine_pw_simps)
-  done
+thm Prim5.upd_Q\<pi>_loop3_def
+term Prim5.upd_Q\<pi>_loop3
+term HM.hm_assn
+term ial_assn
 
-  
-lemma 
-  assumes REL: "(g2,(g,w))\<in>wu_rel N"
-  assumes PRE2: "u<N"
-  shows "
-  doN { num_adjs \<leftarrow> wu2_adjs_len u g2; nfoldli [0..<num_adjs] c (\<lambda>i s. doN { vd \<leftarrow> wu2_adjs_nth u i g2; f vd s }) s}
-  \<le>
-  doN { xs \<leftarrow> mop_wgraph_adjs g w u; nfoldli xs c f s }"  
-  (is "?LHS \<le> ?RHS")
-proof -
-  from REL have [simp]: "g=wu1_\<alpha>g (wu2_\<alpha> g2)" "w=wu1_\<alpha>w (wu2_\<alpha> g2)" "N=length g2"
-    by (auto simp: wu_rel_def Let_def)
-  from wu1_adjs_refine[of "wu2_\<alpha> g2" u]
-    and wu2_adjs_refine[of g2 "wu2_\<alpha> g2" u]
-  have "RETURN (g2!u) \<le> mop_wgraph_adjs (wu1_\<alpha>g (wu2_\<alpha> g2)) (wu1_\<alpha>w (wu2_\<alpha> g2)) u"
-    using REL PRE2
-    by (auto 
-      simp: in_br_conv wu2_adjs_len_def wu2_adjs_def 
-      simp: wu_rel_def Let_def
-      simp: pw_le_iff refine_pw_simps
-      )
-  hence "nfoldli [0..<length (g2!u)] c (\<lambda>i s. do {
-                                    _ \<leftarrow> ASSERT (i < length (g2!u));
-                                    let x = g2!u!i;
-                                    f x s
-                                  }) s \<le> ?RHS" (is "?INT1 \<le> _")
-    apply (rewrite in "_ \<le> \<hole>" nfoldli_by_idx)
-    by (auto simp: pw_le_iff refine_pw_simps)
-  moreover have "?LHS \<le> ?INT1" using PRE2
-    by (auto simp: wu2_adjs_len_def wu2_adjs_nth_def)
-  ultimately show ?thesis by simp
-qed
-  
-    
-  
-    
-lemma 
-  assumes EQ: "g = wu1_\<alpha>g (wu2_\<alpha> g2)" "w=wu1_\<alpha>w (wu2_\<alpha> g2)"
-  assumes I: "wu1_invar (wu2_\<alpha> g2)" "wu2_invar g2"
-  assumes PRE2: "u<length g2"
-  shows "
-  doN { num_adjs \<leftarrow> wu2_adjs_len u g2; nfoldli [0..<num_adjs] c (\<lambda>i s. doN { vd \<leftarrow> wu2_adjs_nth u i g2; f vd s }) s}
-  \<le>
-  doN { xs \<leftarrow> mop_wgraph_adjs g w u; nfoldli xs c f s }"  
-  (is "?LHS \<le> ?RHS")
-  proof -
-    from wu1_adjs_refine[OF I(1), of u] wu2_adjs_refine[of g2 "wu2_\<alpha> g2", OF _ PRE2] I(2)
-    have "RETURN (g2!u) \<le> mop_wgraph_adjs (wu1_\<alpha>g (wu2_\<alpha> g2)) (wu1_\<alpha>w (wu2_\<alpha> g2)) u"
-      by (auto simp: in_br_conv wu2_adjs_len_def wu2_adjs_def pw_le_iff refine_pw_simps)
-    hence "nfoldli [0..<length (g2!u)] c (\<lambda>i s. do {
-                                      _ \<leftarrow> ASSERT (i < length (g2!u));
-                                      let x = g2!u!i;
-                                      f x s
-                                    }) s \<le> ?RHS" (is "?INT1 \<le> _")
-      apply (rewrite in "_ \<le> \<hole>" nfoldli_by_idx)
-      by (auto simp: EQ pw_le_iff refine_pw_simps)
-    moreover have "?LHS \<le> ?INT1"                                          
-      by (auto simp: wu2_adjs_len_def PRE2 wu2_adjs_nth_def)
-    ultimately show ?thesis by simp
-  qed
+thm intf_of_assn
 
-  thm wu1_adjs_refine[OF I(1), of u] wu2_adjs_refine[of g2 "wu2_\<alpha> g2", OF _ PRE2] I(2)
-    
-  
-  apply (rule bind_refine'[where R=Id and R'="{(l,xs). length xs = l}", simplified])
-  subgoal
-    using wu1_adjs_refine[OF I(1), of u] wu2_adjs_refine[of g2 "wu2_\<alpha> g2", OF _ PRE2] I(2)
-    by (auto simp: in_br_conv wu2_adjs_len_def wu2_adjs_def pw_le_iff refine_pw_simps)
-  subgoal for num_adjs adjs  
-    thm nfoldli_mono
-    apply clarsimp
-    apply (rule nfoldli_mono)
-    apply (clarsimp simp: wu2_adjs_nth_def PRE2 wu2_adjs_len_def)
-    
-    
-    using wu2_adjs_refine[of g2 "wu2_\<alpha> g2", OF _ PRE2] I(2)
-    apply (auto simp: pw_le_iff refine_pw_simps)
-    
-  done
+find_theorems intf_of_assn
+
+lemma upd_Q\<pi>_loop4_aux1: "a<b \<Longrightarrow> (bi,b)\<in>snat_rel' TYPE('l::len2) \<Longrightarrow> Suc a < max_snat LENGTH('l)"
+  by (simp add: less_trans_Suc)
+
+
+sepref_definition upd_Q\<pi>_loop4 is "uncurry4 (Prim5.upd_Q\<pi>_loop3)"
+  :: "[\<lambda>((((r,g),u),Q),\<pi>). N = wu2_max g ]\<^sub>a snat64_assn\<^sup>k *\<^sub>a wu3_64_assn\<^sup>k *\<^sub>a snat64_assn\<^sup>k *\<^sub>a (hm_assn' TYPE(64) N)\<^sup>d *\<^sub>a (snat_am_assn' TYPE(64) N)\<^sup>d 
+    \<rightarrow>  hm_assn' TYPE(64) N \<times>\<^sub>a snat_am_assn' TYPE(64) N"
+  unfolding Prim5.upd_Q\<pi>_loop3_def nfoldli_upt_by_while PR_CONST_def Prim5.N_def
+  apply (annot_snat_const "TYPE(64)")
+  supply [simp] = less_trans_Suc upd_Q\<pi>_loop4_aux1[where 'l=64, simplified]
+  supply [[goals_limit = 1]]
+  by sepref
   
   
-    thm conc_trans
-    find_theorems "\<Down>_" name: mono
+sepref_register Prim5.upd_Q\<pi>_loop3 :: "nat
+     \<Rightarrow> (nat \<times> nat) list list
+        \<Rightarrow> nat \<Rightarrow> ((nat, nat) i_map) \<Rightarrow> ((nat, nat) i_map) \<Rightarrow> (((nat, nat) i_map) \<times> ((nat, nat) i_map)) nres"
   
+lemmas [sepref_fr_rules] = upd_Q\<pi>_loop4.refine
+term Prim5.prim5
+
+lemma eval_wu2max_bind_aux: 
+  "bind_ref_tag x (RETURN $ (wu2_max $ b)) \<Longrightarrow> x = wu2_max b" by (auto simp: bind_ref_tag_def)
+
+
+sepref_definition prim6 is "uncurry Prim5.prim5" 
+  :: "snat64_assn\<^sup>k *\<^sub>a wu3_64_assn\<^sup>k \<rightarrow>\<^sub>a\<^sub>d (\<lambda>(r,g). hm_assn' TYPE(64) (wu2_max g) \<times>\<^sub>a snat_am_assn' TYPE(64) (wu2_max g))"
+  unfolding Prim5.prim5_def Prim5.N_def
+  apply (annot_snat_const "TYPE(64)")
+  apply sepref_dbg_keep
+  apply sepref_dbg_trans_step
+  apply sepref_dbg_trans_step
+  apply sepref_dbg_trans_step
+  apply (frule eval_wu2max_bind_aux, hypsubst)
+  apply sepref_dbg_trans_step
+  apply sepref_dbg_trans_step
+  apply sepref_dbg_trans_step
+  apply sepref_dbg_trans_step
+  apply sepref_dbg_trans_step
+  apply sepref_dbg_trans_step
+  apply sepref_dbg_trans_step
+  apply sepref_dbg_trans_step
+  apply sepref_dbg_trans_step
+  apply sepref_dbg_trans_step
+  apply sepref_dbg_trans_step
+  apply sepref_dbg_trans_step
+  apply sepref_dbg_trans_step
+  apply sepref_dbg_trans_step
+  apply sepref_dbg_trans_step
+  apply sepref_dbg_trans_step
+  oops sorry
+  xxx, ctd here
+  apply sepref_dbg_trans_step
+  apply sepref_dbg_trans_step
+  apply sepref_dbg_trans_step
+  apply sepref_dbg_trans_step
+  apply sepref_dbg_trans_step
+  apply sepref_dbg_trans_step
+  apply sepref_dbg_trans_step
   
-    apply (auto simp: wu2_adjs_len_def)
-  
-  
-  
-  thm bind_refine[where R=Id, simplified]
-  apply (rule bind_mono)
-  
-  thm wu1_adjs_refine[OF I(1)]
   
   
   oops
-  xxx: Build prototype setoid rewriter!
+  apply sepref_dbg_trans_step_keep
+  apply sepref_dbg_frame
+  apply sepref_dbg_frame_step_keep
+  apply sepref_dbg_trans_step
+  apply sepref_dbg_trans_step
+  
+  oops
+  apply sepref_dbg_trans_step_keep
+  
+  find_in_thms HM.mop_hm_empty_fixed in sepref_fr_rules
   
   
-  unfolding wu2_adjs_len_def
-  
-  find_theorems wu1_adjs
-  find_theorems mop_wgraph_adjs
-  
-  
-find_theorems nfoldli "[_..<_]"
+  oops
+  xxx, id problem. First guess: custom map-inits!?
 
-thm nfoldli_by_idx  
-  
-  
-oops  
-    
-xxx: Refine iteration over adjacent nodes by for-loop!
-  
-  
-context 
-  fixes VL :: "'vl::len2 itself"
-  fixes WL :: "'wl::len2 itself"
-begin  
 
-  private abbreviation (input) "V_assn \<equiv> snat_assn' TYPE('vl)"
-  private abbreviation (input) "W_assn \<equiv> snat_assn' TYPE('wl)"
-  private abbreviation (input) "wu3_assn \<equiv> aal_assn' TYPE('vl) TYPE('vl) (V_assn \<times>\<^sub>a W_assn)"
-  
-  sepref_definition wu3_empty is "RETURN o wu2_empty" 
-    :: "[\<lambda>_. 4<LENGTH('vl)]\<^sub>a (snat_assn' TYPE('vl))\<^sup>k \<rightarrow> wu3_assn"
-    unfolding wu2_empty_def
-    apply (rewrite aal_fold_custom_empty)
-    by sepref
-    
-  sepref_definition wu3_ins_edge is "uncurry2 wu2_ins_edge" 
-    :: "(V_assn \<times>\<^sub>a V_assn)\<^sup>k *\<^sub>a W_assn\<^sup>k *\<^sub>a wu3_assn\<^sup>d \<rightarrow>\<^sub>a wu3_assn"
-    unfolding wu2_ins_edge_def
-    supply [dest!] = rdomp_aal_assnD
-    by sepref
-    
-  sepref_definition wu3_adjs_len is "uncurry wu2_adjs_len"  
-    :: "V_assn\<^sup>k *\<^sub>a wu3_assn\<^sup>k \<rightarrow>\<^sub>a V_assn"
-    unfolding wu2_adjs_len_def
-    by sepref
-    
-  sepref_definition wu3_adjs_nth is "uncurry2 wu2_adjs_nth"  
-    :: "V_assn\<^sup>k *\<^sub>a V_assn\<^sup>k *\<^sub>a wu3_assn\<^sup>k \<rightarrow>\<^sub>a V_assn\<times>\<^sub>aW_assn"
-    unfolding wu2_adjs_nth_def
-    by sepref
-    
+
+sepref_definition upd_Q\<pi>_loop4 is "uncurry4 Prim5.upd_Q\<pi>_loop3"
+  :: "snat64_assn\<^sup>k *\<^sub>a wu3_assn\<^sup>k *\<^sub>a snat64_assn\<^sup>k *\<^sub>a (hm_assn' TYPE(64))  "
+
+
+oops
+xxx: we need translation or nfoldli to for-loop!
+
+ 
+            
+oops
+
+
+
+oops
+again: Prototype setoid rewrite:
+        
+for boolean, show \<Longrightarrow>
+use mono-lemmas
+
+
+   ?a'\<le>a  b\<le>?b'
+------------------  (init-rule)
+      a\<le>b
+
+ m\<le>m'  f\<le>f'
+------------------------ (bind-rule)     
+ bind m f \<le> bind m' f'
+
+ 
+  R \<subseteq> R'  f \<le> f'
+-------------------- (conc-rule)
+   \<Down>R f \<le> \<Down>R' f'
+ 
+     -
+------------ (exit-rule)  
+  x \<le> x 
+   
+   
     
     find_theorems rdomp
     
